theories/zoo_saturn/ws_queue_2__opaque.v
@@ -2,6 +2,8 @@ From zoo_saturn Require Import
   ws_queue_2__code.
 
 #[global] Opaque ws_queue_2_create.
+#[global] Opaque ws_queue_2_size.
+#[global] Opaque ws_queue_2_is_empty.
 #[global] Opaque ws_queue_2_push.
 #[global] Opaque ws_queue_2_pop.
 #[global] Opaque ws_queue_2_steal.
